Coq/src/SimRelAddEW.v
@@ -118,7 +118,115 @@ Section SimRelAddEW.
     ⟪ wE' : SE S' w' ⟫ /\
     ⟪ wW' : SW S' w' ⟫ /\
     ⟪ wsE2A : e2a S' □₁ ws ⊆₁ eq (e2a S' w') ⟫ /\
-    ⟪ wsI : ws ⊆₁ dom_rel ((Sew S)^? ⨾ ⦗ h □₁ I ⦘) ⟫ /\
+    ⟪ wsI : ws ⊆₁ dom_rel ((Sew S)^? ⨾ ⦗ f □₁ I ⦘) ⟫ /\
     ⟪ EW' : Sew S' ≡ Sew S ∪ ESstep.ew_delta ws w' ⟫. 
+
+  Section SimRelAddEWProps. 
+
+    Lemma sim_add_ew_wsE ws w' k S S' 
+          (st st' st'' : thread_st (ES.cont_thread S k))
+          (SRCC : simrel_cert prog S G sc TC f TC' h k st st'') 
+          (SAEW : sim_add_ew ws w' S S') :
+      ws ⊆₁ SE S.
+    Proof. 
+      cdes SAEW.
+      assert (ES.Wf S) as WFS.
+      { apply SRCC. }
+      etransitivity; [apply wsI|].
+      rewrite crE. relsf. split.
+      { etransitivity. 
+        2 : { eapply a2e_img. apply SRCC.(sim_com). }
+        basic_solver 10. }
+      rewrite ES.ewE; auto. basic_solver.
+    Qed.
+
+    Lemma sim_add_ew_ws_same_lab ws w' k S S' 
+          (st st' st'' : thread_st (ES.cont_thread S k))
+          (SRCC : simrel_cert prog S G sc TC f TC' h k st st'') 
+          (SAEW : sim_add_ew ws w' S S') :
+      (Glab ∘ e2a S') □₁ ws ⊆₁ eq ((Glab ∘ (e2a S')) w').
+    Proof. 
+      cdes SAEW.
+      unfold compose. 
+      intros a [x [WSx LABx]]. subst a.
+      arewrite (e2a S' x = e2a S' w'); auto.
+      erewrite wsE2A; eauto.
+      basic_solver.
+    Qed.
+
+    Lemma weaken_sim_add_ew ws w' k k' e e' S S' 
+          (st st' st'' : thread_st (ES.cont_thread S k))
+          (SRCC : simrel_cert prog S G sc TC f TC' h k st st'') 
+          (BSTEP_ : ESBasicStep.t_ (thread_lts (ES.cont_thread S k)) k k' st st' e e' S S') 
+          (SAEW : sim_add_ew ws w' S S') 
+          (CST_REACHABLE : (lbl_step (ES.cont_thread S k))＊ st' st'') 
+          (wEE' : (eq e ∪₁ eq_opt e') w') : 
+      ESstep.add_ew ws w' S S'.
+    Proof. 
+      cdes BSTEP_; cdes SAEW.
+      assert (ESBasicStep.t e e' S S') as BSTEP.
+      { econstructor. eauto. }
+      assert (ES.Wf S) as WFS.
+      { apply SRCC. }
+      
+      constructor; splits; auto.
+      (* wsE : ws ⊆₁ E S *)
+      { eapply sim_add_ew_wsE; eauto. }
+      (* wsW : ws ⊆₁ W S *)
+      { etransitivity; [apply wsI|]. 
+        rewrite crE. relsf. split.
+        { intros x [a [Ia EQa]]. subst x.
+          unfold is_w. 
+          fold (compose (Slab S) f a).
+          erewrite flab; [| apply SRCC | basic_solver].
+          fold (is_w Glab a).
+          eapply issuedW; eauto.
+          apply SRCC. }
+        rewrite ES.ewD; auto. basic_solver. }
+      (* LOCWS : ws ⊆₁ same_loc S' w' *)
+      { intros x WSx.
+        assert ((restr_rel (SE S') (same_loc (Slab S'))) w' x)
+          as HH. 
+        { eapply same_lab_u2v_dom_same_loc.
+          { eapply basic_step_e2a_same_lab_u2v; eauto; apply SRCC. }
+          unfolder; splits; eauto.
+          { unfold same_loc, loc. 
+            erewrite sim_add_ew_ws_same_lab; eauto.
+            basic_solver. }
+          eapply ESBasicStep.basic_step_acts_set_mon; eauto. 
+          eapply sim_add_ew_wsE; eauto. }
+        unfolder in HH. desf. } 
+      (* VALWS : ws ⊆₁ same_val S' w' *)
+      { intros x WSx.
+        destruct 
+          (excluded_middle_informative (I (e2a S' w')))
+          as [Iw' | nIw'].
+        { admit. }
+        exfalso. apply nIw'. 
+        edestruct wsI as [y wsIy]; eauto.
+        destruct wsIy as [z [[EQxz | EW] [EQyz [a [Ia EQa]]]]].
+        { subst x y z. 
+          erewrite wsE2A; eauto.
+          unfolder; eexists; splits; eauto.
+          erewrite basic_step_e2a_eq_dom; eauto.
+          { eapply a2e_fix. 
+            { apply SRCC.(sim_com). }
+            basic_solver 10. }
+          eapply a2e_img.
+          { apply SRCC.(sim_com). }
+          basic_solver 10. }
+        subst y z. 
+        erewrite wsE2A; eauto.
+        unfolder; eexists; splits; eauto.
+        erewrite basic_step_e2a_eq_dom; eauto.
+        { etransitivity. 
+          { eapply e2a_ew; [apply SRCC|].
+            basic_solver 10. }
+          eapply a2e_fix. 
+          { apply SRCC.(sim_com). }
+          basic_solver 10. }
+        apply ES.ewE, seq_eqv_lr in EW; desf. }
+      all : admit. 
+    Admitted.
 
 End SimRelAddEW.
